src/IO.thy
@@ -1,8 +1,8 @@
 theory IO
-  imports Main "HOL-Library.Countable" "HOL-Library.State_Monad"
+  imports Main "HOL-Library.Countable" "HOL-Library.Monad_Syntax"
 begin
-
-class repr = countable
+                              
+class repr = countable + typerep
 
 instance nat :: repr ..
 instance unit :: repr ..
@@ -12,7 +12,7 @@ instance int :: repr ..
 type_synonym addr = nat
 
 record world =
-  memory :: "addr \<Rightarrow> nat"
+  memory :: "addr \<Rightarrow> typerep"
   used :: "addr"
 
 definition empty_world :: "world" where
@@ -21,21 +21,36 @@ definition empty_world :: "world" where
 datatype 'a ref = Ref addr
 datatype 'a array = Array addr nat
 
-datatype 'a io = IO (run_io: "(world, 'a) state")
+datatype 'a io = IO (run_io: "world \<Rightarrow> 'a \<times> world")
 
 definition return :: "'a \<Rightarrow> 'a io" where
-  "return x = IO (State_Monad.return x)"
+  "return x = IO (\<lambda>w. (x,w))"
 
 definition bind :: "'a io \<Rightarrow> ('a \<Rightarrow> 'b io) \<Rightarrow> 'b io" where
-  "bind x f = IO (run_io x \<bind> (run_io \<circ> f))"
+  "bind x f = IO (\<lambda>w. case run_io x w of (y,w') \<Rightarrow> run_io (f y) w')"
 
 adhoc_overloading
   Monad_Syntax.bind IO.bind
 
+(* IO monad *)
+
+lemma monad_left_id[simp]: "return a \<bind> f = f a"
+  apply (simp add: return_def bind_def)
+  done
+
+lemma monad_right_id[simp]: "m \<bind> return = m"
+  apply (simp add: return_def bind_def)
+  done
+
+lemma monad_assoc[simp]:
+  fixes m :: "'a io"
+  shows "(m \<bind> f) \<bind> g = m \<bind> (\<lambda>x. f x \<bind> g)"
+  unfolding bind_def by (auto split: prod.splits)
+
 fun new_world :: "'a::repr \<Rightarrow> world \<Rightarrow> 'a ref \<times> world" where
   "new_world val w = (
     let newAddr = used w in
-    ( Ref newAddr, \<lparr> memory = \<lambda>i. if i = newAddr then to_nat val else memory w i, used = newAddr + 1 \<rparr> )
+    ( Ref newAddr, \<lparr> memory = \<lambda>i. if i = newAddr then typerep_of nat else memory w i, used = newAddr + 1 \<rparr> )
   )"
 
 fun alloc_world :: "nat \<Rightarrow> world \<Rightarrow> 'a array \<times> world" where
@@ -45,7 +60,7 @@ fun alloc_world :: "nat \<Rightarrow> world \<Rightarrow> 'a array \<times> worl
 
 fun get_world :: "addr \<Rightarrow> world \<Rightarrow> 'a::repr \<times> world" where
   "get_world addr w = (
-    ( from_nat (memory w addr), w )
+    ( TYPEREP('a) (from_nat (memory w addr)), w )
   )"
 
 fun put_world :: "addr \<Rightarrow> 'a::repr \<Rightarrow> world \<Rightarrow> unit \<times> world" where
@@ -54,22 +69,22 @@ fun put_world :: "addr \<Rightarrow> 'a::repr \<Rightarrow> world \<Rightarrow> 
   )"
 
 fun new :: "'a::repr \<Rightarrow> 'a ref io" where
-  "new val = IO (State (new_world val))"
+  "new val = IO (new_world val)"
 
 fun get :: "'a ref \<Rightarrow> 'a::repr io" where
-  "get (Ref ref) = IO (State (get_world ref))"
+  "get (Ref ref) = IO (get_world ref)"
 
 fun put :: "'a ref \<Rightarrow> 'a::repr \<Rightarrow> unit io" where
-  "put (Ref ref) val = IO (State (put_world ref val))"
+  "put (Ref ref) val = IO (put_world ref val)"
 
 fun new_array :: "nat \<Rightarrow> ('a array) io" where
-  "new_array s = IO (State (alloc_world s))"
+  "new_array s = IO (alloc_world s)"
 
 fun read_array :: "'a array \<Rightarrow> nat \<Rightarrow> 'a::repr io" where
-  "read_array (Array arr _) i = IO (State (get_world (arr + i)))"
+  "read_array (Array arr _) i = IO (get_world (arr + i))"
 
 fun write_array :: "'a array \<Rightarrow> nat \<Rightarrow> 'a::repr \<Rightarrow> unit io" where
-  "write_array (Array arr _) i val = IO (State (put_world (arr + i) val))"
+  "write_array (Array arr _) i val = IO (put_world (arr + i) val)"
 
 fun swap_array :: "'a::repr array \<Rightarrow> nat \<Rightarrow> nat \<Rightarrow> unit io" where
   "swap_array arr i j = do {
@@ -79,6 +94,11 @@ fun swap_array :: "'a::repr array \<Rightarrow> nat \<Rightarrow> nat \<Rightarr
     write_array arr i valJ;
     return ()
   }"
+
+(* IO Operations *)
+lemma get_set[simp]: "get ref \<bind> put ref = return ()"
+  apply (cases ref)
+  unfolding bind_def return_def apply simp
 
 (* Monadic Combinators *)
 
@@ -113,21 +133,5 @@ code_printing
   | constant forMu \<rightharpoonup> (Haskell) "forM_"
   | constant mapM \<rightharpoonup> (Haskell) "mapM_"
   | constant whenu \<rightharpoonup> (Haskell) "when"
-
-(* IO monad *)
-
-lemma monad_left_id: "return a \<bind> f = f a"
-  apply (simp add: return_def bind_def comp_def)
-  done
-
-lemma monad_right_id: "m \<bind> return = m"
-  apply (simp add: return_def bind_def comp_def)
-  done
-
-lemma monad_assoc:
-  fixes m :: "'a io"
-  shows "(m \<bind> f) \<bind> g = m \<bind> (\<lambda>x. f x \<bind> g)"
-  apply (simp add: return_def bind_def comp_def)
-  done
 
 end
